theories/typechecker/typechecker.v
@@ -1,0 +1,226 @@
+Require Import RecordUpdate.RecordUpdate.
+From stdpp Require Import base list.
+From Stdlib.Strings Require Import String.
+
+From RichWasm Require Import layout syntax typing util.
+Set Bullet Behavior "Strict Subproofs".
+
+Definition type_error := string.
+Definition ok := unit.
+Definition type_checker_res := sum ok type_error.
+
+Definition ok_term : type_checker_res := inl ().
+Definition INR (s:string) : type_checker_res := inr s.
+
+
+
+(* No matter how type_checker_res changes, this MUST stay the same *)
+Definition check_ok In (func: In -> type_checker_res) (i: In) : bool :=
+  match (func i) with
+  | inl a => true
+  | inr a => false
+  end.
+
+Definition check_ok_output (res: type_checker_res) : bool :=
+  match res with
+  | inl a => true
+  | inr a => false
+  end.
+
+(* This is only true if ok is kept at unit. Unfortunately most of the proofs
+ rely on this. *)
+Lemma check_ok_true_to_prop In (func: In -> type_checker_res) (i:In) :
+  check_ok In func i = true -> func i = ok_term.
+Proof.
+  intros. unfold ok_term.
+  destruct (func i) eqn:H'.
+  - unfold ok in o.
+    assert (o = tt) by (by destruct o).
+    subst; auto.
+  - unfold check_ok in H.
+    rewrite H' in H. inversion H.
+Qed.
+Lemma check_ok_output_true_to_prop (res: type_checker_res) :
+  check_ok_output res = true -> res = ok_term.
+Proof.
+  intros. unfold ok_term.
+  destruct (res) eqn:H'.
+  - unfold ok in o.
+    assert (o = tt) by (by destruct o).
+    subst; auto.
+  - unfold check_ok in H.
+    simpl in H.
+    inversion H.
+Qed.
+
+(* Helper function for converting between forall inductive hyp and foldr boolean version *)
+Lemma Forall_foldr_bool_to_prop A (Pprop : A -> Prop) (Pbool : A -> bool) (l : list A) :
+  (Forall (λ x:A, (Pbool x = true) -> Pprop x) l) ->
+  (foldr (λ x:A, andb (Pbool x)) true l) = true ->
+  Forall Pprop l.
+Proof.
+  intros HForall Hfoldr.
+  apply Forall_fold_right.
+  induction l; simpl; auto.
+  - rewrite foldr_cons in Hfoldr; apply andb_prop in Hfoldr as [a_true l_true].
+    apply Forall_cons_1 in HForall; destruct HForall as [a_prop l_prop].
+    split; auto.
+Qed.
+
+(* Converting between _ = ok_term to check_ok = true *)
+Lemma equal_okterm_to_checkok In (func: In -> type_checker_res) (Pbool : In -> Prop) :
+  forall i:In,
+    ((func i = ok_term -> Pbool i) ->
+     (check_ok In func i = true -> Pbool i)).
+Proof.
+  intros. apply H.
+  by apply check_ok_true_to_prop.
+Qed.
+
+
+
+
+(** WE BEGIN **)
+
+
+(* mem_ok *)
+Definition mem_ok_checker (k:kind_ctx) (mem:memory) : type_checker_res :=
+  match mem with
+  | BaseM cm => ok_term
+  | VarM m =>
+      if m <? k.(kc_mem_vars) then ok_term else INR "mem_ok error"
+  end.
+
+Lemma mem_ok_checker_correct (k:kind_ctx) (mem:memory) :
+  (mem_ok_checker k mem = ok_term) -> mem_ok k mem.
+Proof.
+  intros.
+  destruct mem.
+  - apply OKVarM.
+    simpl in H.
+    destruct (n <? kc_mem_vars k) eqn:H'.
+    + apply Nat.ltb_lt in H'. auto.
+    + inversion H.
+  - apply OKBaseM.
+Qed.
+
+
+
+(* rep_ok *)
+Fixpoint rep_ok_checker (k:kind_ctx) (rep:representation) : type_checker_res :=
+  match rep with
+  | AtomR ι => ok_term
+  | VarR r => if r <? k.(kc_rep_vars) then ok_term else INR "rep_ok error"
+  | ProdR ρs =>
+      if (foldr (λ i:representation, andb (check_ok representation (rep_ok_checker k) i)) true ρs)
+           then ok_term else INR "rep_ok error"
+  | SumR ρs =>
+       if (foldr (λ i:representation, andb (check_ok representation (rep_ok_checker k) i)) true ρs)
+           then ok_term else INR "rep_ok error"
+ end.
+
+Lemma rep_ok_checker_correct (k:kind_ctx) (rep:representation) :
+  (rep_ok_checker k rep = ok_term) -> rep_ok k rep.
+Proof.
+  intros.
+  induction rep using rep_ind.
+  - apply OKVarR.
+    simpl in H.
+    destruct (idx <? kc_rep_vars k) eqn:H'.
+    + apply Nat.ltb_lt in H'. auto.
+    + inversion H.
+  - apply OKSumR.
+    simpl in H.
+    destruct (foldr (λ i:representation, andb (check_ok representation (rep_ok_checker k) i)) true ρs) eqn:H'.
+    + clear H.
+      apply (Forall_impl _ (λ x, check_ok representation (rep_ok_checker k) x = true -> rep_ok k x)) in H0.
+      * eapply Forall_foldr_bool_to_prop; [apply H0 | apply H'].
+      * apply equal_okterm_to_checkok.
+    + inversion H.
+  - apply OKProdR.
+    simpl in H.
+    destruct (foldr (λ i:representation, andb (check_ok representation (rep_ok_checker k) i)) true ρs) eqn:H'.
+    + clear H.
+      apply (Forall_impl _ (λ x, check_ok representation (rep_ok_checker k) x = true -> rep_ok k x)) in H0.
+      * eapply Forall_foldr_bool_to_prop; [apply H0 | apply H'].
+      * apply equal_okterm_to_checkok.
+    + inversion H.
+  - apply OKAtomR.
+Qed.
+
+
+
+(* size_ok *)
+Fixpoint size_ok_checker (k:kind_ctx) (s:size) : type_checker_res :=
+  match s with
+  | ConstS n => ok_term
+  | VarS r => if r <? k.(kc_size_vars) then ok_term else INR "size_ok error"
+  | RepS ρ => match (rep_ok_checker k ρ) with
+              | inl _ => ok_term
+              | err => err (* this allows propagation*)
+                         (* you could also just ret rep_ok_checker. Idk which would be
+                          better for future changeability. I'll do just ret later*)
+              end
+  | SumS σs =>
+      if (foldr (λ i:size, andb (check_ok size (size_ok_checker k) i)) true σs)
+           then ok_term else INR "size_ok error"
+  | ProdS σs =>
+      if (foldr (λ i:size, andb (check_ok size (size_ok_checker k) i)) true σs)
+           then ok_term else INR "size_ok error"
+  end.
+
+Lemma size_ok_checker_correct (k:kind_ctx) (s:size) :
+  (size_ok_checker k s = ok_term) -> size_ok k s.
+Proof.
+  intros.
+  induction s using size_ind.
+  - apply OKVarS.
+    simpl in H.
+    destruct (idx <? kc_size_vars k) eqn:H'.
+    + apply Nat.ltb_lt in H'. auto.
+    + inversion H.
+  - apply OKSumS.
+    simpl in H.
+    destruct (foldr (λ i:size, andb (check_ok size (size_ok_checker k) i)) true σs) eqn:H'.
+    + clear H.
+      apply (Forall_impl _ (λ x, check_ok size (size_ok_checker k) x = true -> size_ok k x)) in H0.
+      * eapply Forall_foldr_bool_to_prop; [apply H0 | apply H'].
+      * apply equal_okterm_to_checkok.
+    + inversion H.
+  - apply OKProdS.
+    simpl in H.
+    destruct (foldr (λ i:size, andb (check_ok size (size_ok_checker k) i)) true σs) eqn:H'.
+    + clear H.
+      apply (Forall_impl _ (λ x, check_ok size (size_ok_checker k) x = true -> size_ok k x)) in H0.
+      * eapply Forall_foldr_bool_to_prop; [apply H0 | apply H'].
+      * apply equal_okterm_to_checkok.
+    + inversion H.
+  - apply OKRepS.
+    simpl in H.
+    destruct (rep_ok_checker k ρ) eqn:H'.
+    + apply rep_ok_checker_correct.
+      unfold ok in o.
+      assert (o = tt) by (by destruct o).
+      subst; auto.
+    + inversion H.
+  - apply OKConstS.
+Qed.
+
+
+(* kind_ok *)
+Definition kind_ok_checker (k:kind_ctx) (ki: kind) : type_checker_res :=
+  match ki with
+  | (VALTYPE ρ χ δ) => rep_ok_checker k ρ
+  | MEMTYPE σ δ => size_ok_checker k σ
+  end.
+
+Lemma kind_ok_checker_correct (k:kind_ctx) (ki:kind) :
+  (kind_ok_checker k ki = ok_term) -> kind_ok k ki.
+Proof.
+  intros.
+  destruct ki; simpl in H.
+  - apply OKVALTYPE.
+    apply rep_ok_checker_correct; auto.
+  - apply OKMEMTYPE.
+    apply size_ok_checker_correct; auto.
+Qed.
